compiler/examples/gimli/proofs/gimli_ct.ec
@@ -4,11 +4,11 @@ require Gimli_x86_ct Gimli_arm_ct Gimli_avx_ct.
   * Since it is an address, its value is leaked, and should be public. *)
 
 equiv gimli_x86_ct :
-  Gimli_x86_ct.M.gimli ~ Gimli_x86_ct.M.gimli : true ==> res{1}.`2 = res{2}.`2.
+  Gimli_x86_ct.M.gimli ~ Gimli_x86_ct.M.gimli : true ==> res{1}.`1 = res{2}.`1.
 proof. proc; inline *; sim: (={leak}). qed.
 
 equiv gimli_arm_ct :
-  Gimli_arm_ct.M.gimli ~ Gimli_arm_ct.M.gimli : true  ==> res{1}.`2 = res{2}.`2.
+  Gimli_arm_ct.M.gimli ~ Gimli_arm_ct.M.gimli : true  ==> res{1}.`1 = res{2}.`1.
 proof. proc; inline *; sim: (={leak}). qed.
 
 equiv gimli_avx_ct :
